books/projects/async/fifo/queue3.lisp
@@ -4,7 +4,7 @@
 ;; ACL2.
 
 ;; Cuong Chau <ckcuong@cs.utexas.edu>
-;; February 2018
+;; April 2018
 
 (in-package "ADE")
 
@@ -19,7 +19,7 @@
 ;;; Table of Contents:
 ;;;
 ;;; 1. DE Module Generator of Q3
-;;; 2. Specifying the Final State of Q3 After An N-Step Execution
+;;; 2. Specify the Final State of Q3 After An N-Step Execution
 ;;; 3. Single-Step-Update Property
 ;;; 4. Relationship Between the Input and Output Sequences
 
@@ -27,8 +27,8 @@
 
 ;; 1. DE Module Generator of Q3
 ;;
-;; Constructing a DE module generator for a queue of three links, Q3, using the
-;; link-joint model. Proving the value and state lemmas for this module
+;; Construct a DE module generator for a queue of three links, Q3, using the
+;; link-joint model.  Prove the value and state lemmas for this module
 ;; generator.
 
 (defconst *queue3$go-num* 4)
@@ -44,8 +44,7 @@
   (+ (queue3$data-ins-len data-width)
      *queue3$go-num*))
 
-;; DE module generator of Q3. It reports the "in-act" signal at its input port,
-;; and the "out-act" signal and output data at its output port.
+;; DE module generator of Q3
 
 (module-generator
  queue3* (data-width)
@@ -125,7 +124,7 @@
  `(progn
     ,@(state-accessors-gen 'queue3 '(l0 d0 l1 d1 l2 d2) 0)))
 
-;; DE netlist generator. A generated netlist will contain an instance of Q3.
+;; DE netlist generator.  A generated netlist will contain an instance of Q3.
 
 (defun queue3$netlist (data-width)
   (declare (xargs :guard (natp data-width)))
@@ -203,6 +202,189 @@
   :hints (("Goal" :in-theory (enable queue3$valid-st)))
   :rule-classes :forward-chaining)
 
+;; Extract the input and output signals from Q3
+
+(progn
+  ;; Extract the input data
+
+  (defun queue3$data-in (inputs data-width)
+    (declare (xargs :guard (and (true-listp inputs)
+                                (natp data-width))))
+    (take (mbe :logic (nfix data-width)
+               :exec  data-width)
+          (nthcdr 2 inputs)))
+
+  (defthm len-queue3$data-in
+    (equal (len (queue3$data-in inputs data-width))
+           (nfix data-width)))
+
+  (in-theory (disable queue3$data-in))
+
+  ;; Extract the "in-act" signal
+
+  (defund queue3$in-act (inputs st data-width)
+    (b* ((full-in (nth 0 inputs))
+         (go-signals (nthcdr (queue3$data-ins-len data-width) inputs))
+         (go-in (nth 0 go-signals))
+
+         (l0 (get-field *queue3$l0* st)))
+      (joint-act full-in (car l0) go-in)))
+
+  ;; Extract the "out-act" signal
+
+  (defund queue3$out-act (inputs st data-width)
+    (b* ((empty-out- (nth 1 inputs))
+         (go-signals (nthcdr (queue3$data-ins-len data-width) inputs))
+         (go-out (nth 3 go-signals))
+
+         (l2 (get-field *queue3$l2* st)))
+      (joint-act (car l2) empty-out- go-out)))
+
+  ;; Extract the output data
+
+  (defund queue3$data-out (st)
+    (v-threefix (strip-cars (get-field *queue3$d2* st))))
+
+  (defthm len-queue3$data-out-1
+    (implies (queue3$st-format st data-width)
+             (equal (len (queue3$data-out st))
+                    data-width))
+    :hints (("Goal" :in-theory (enable queue3$st-format
+                                       queue3$data-out))))
+
+  (defthm len-queue3$data-out-2
+    (implies (queue3$valid-st st data-width)
+             (equal (len (queue3$data-out st))
+                    data-width))
+    :hints (("Goal" :in-theory (enable queue3$valid-st))))
+
+  (defthm bvp-queue3$data-out
+    (implies (and (queue3$valid-st st data-width)
+                  (queue3$out-act inputs st data-width))
+             (bvp (queue3$data-out st)))
+    :hints (("Goal" :in-theory (enable queue3$valid-st
+                                       queue3$out-act
+                                       queue3$data-out))))
+  )
+
+(not-primp-lemma queue3) ;; Prove that Q3 is not a DE primitive.
+
+;; The value lemma for Q3
+
+(defthmd queue3$value
+  (b* ((inputs (list* full-in empty-out- (append data-in go-signals))))
+    (implies (and (queue3& netlist data-width)
+                  (equal (len data-in) data-width)
+                  (true-listp go-signals)
+                  (equal (len go-signals) *queue3$go-num*)
+                  (queue3$st-format st data-width))
+             (equal (se (si 'queue3 data-width) inputs st netlist)
+                    (list* (queue3$in-act inputs st data-width)
+                           (queue3$out-act inputs st data-width)
+                           (queue3$data-out st)))))
+  :hints (("Goal"
+           :do-not-induct t
+           :do-not '(preprocess)
+           :expand (se (si 'queue3 data-width)
+                       (list* full-in empty-out-
+                              (append data-in go-signals))
+                       st
+                       netlist)
+           :in-theory (e/d (de-rules
+                            not-primp-queue3
+                            queue3&
+                            queue3*$destructure
+                            joint-cntl$value
+                            latch-n$value
+                            v-buf$value
+                            queue3$st-format
+                            queue3$in-act
+                            queue3$out-act
+                            queue3$data-out)
+                           ((queue3*)
+                            de-module-disabled-rules)))))
+
+;; This function specifies the next state of Q3, namely, the next states of
+;; three links L0, L1, and L2.
+
+(defun queue3$step (inputs st data-width)
+  (b* ((data-in    (queue3$data-in inputs data-width))
+       (go-signals (nthcdr (queue3$data-ins-len data-width) inputs))
+
+       (go-trans1 (nth 1 go-signals))
+       (go-trans2 (nth 2 go-signals))
+
+       (l0 (get-field *queue3$l0* st))
+       (d0 (get-field *queue3$d0* st))
+       (l1 (get-field *queue3$l1* st))
+       (d1 (get-field *queue3$d1* st))
+       (l2 (get-field *queue3$l2* st))
+       (d2 (get-field *queue3$d2* st))
+
+       (in-act (queue3$in-act inputs st data-width))
+       (out-act (queue3$out-act inputs st data-width))
+       (trans1-act (joint-act (car l0) (car l1) go-trans1))
+       (trans2-act (joint-act (car l1) (car l2) go-trans2)))
+    (list
+     ;; L0
+     (list (f-sr in-act trans1-act (car l0)))
+     (pairlis$ (fv-if in-act data-in (strip-cars d0))
+               nil)
+
+     ;; L1
+     (list (f-sr trans1-act trans2-act (car l1)))
+     (pairlis$ (fv-if trans1-act (strip-cars d0) (strip-cars d1))
+               nil)
+
+     ;; L2
+     (list (f-sr trans2-act out-act (car l2)))
+     (pairlis$ (fv-if trans2-act (strip-cars d1) (strip-cars d2))
+               nil))))
+
+(defthm len-of-queue3$step
+  (equal (len (queue3$step inputs st data-width))
+         *queue3$st-len*))
+
+;; The state lemma for Q3
+
+(defthmd queue3$state
+  (b* ((inputs (list* full-in empty-out- (append data-in go-signals))))
+    (implies (and (queue3& netlist data-width)
+                  (true-listp data-in)
+                  (equal (len data-in) data-width)
+                  (true-listp go-signals)
+                  (equal (len go-signals) *queue3$go-num*)
+                  (queue3$st-format st data-width))
+             (equal (de (si 'queue3 data-width) inputs st netlist)
+                    (queue3$step inputs st data-width))))
+  :hints (("Goal"
+           :do-not-induct t
+           :do-not '(preprocess)
+           :expand (de (si 'queue3 data-width)
+                       (list* full-in empty-out-
+                              (append data-in go-signals))
+                       st
+                       netlist)
+           :in-theory (e/d (de-rules
+                            not-primp-queue3
+                            queue3&
+                            queue3*$destructure
+                            queue3$st-format
+                            queue3$data-in
+                            queue3$in-act
+                            queue3$out-act
+                            joint-cntl$value
+                            latch-n$value latch-n$state
+                            v-buf$value)
+                           ((queue3*)
+                            de-module-disabled-rules)))))
+
+(in-theory (disable queue3$step))
+
+;; ======================================================================
+
+;; 2. Specify the Final State of Q3 After An N-Step Execution
+
 ;; Q3 simulator
 
 (progn
@@ -248,189 +430,6 @@
           state)))
   )
 
-;; Extracting the input data
-
-(defun queue3$data-in (inputs data-width)
-  (declare (xargs :guard (and (true-listp inputs)
-                              (natp data-width))))
-  (take (mbe :logic (nfix data-width)
-             :exec  data-width)
-        (nthcdr 2 inputs)))
-
-(defthm len-queue3$data-in
-  (equal (len (queue3$data-in inputs data-width))
-         (nfix data-width)))
-
-(in-theory (disable queue3$data-in))
-
-;; Extracting the "in-act" signal
-
-(defund queue3$in-act (inputs st data-width)
-  (b* ((full-in (nth 0 inputs))
-       (go-signals (nthcdr (queue3$data-ins-len data-width) inputs))
-       (go-in (nth 0 go-signals))
-
-       (l0 (get-field *queue3$l0* st)))
-    (joint-act full-in (car l0) go-in)))
-
-;; Extracting the "out-act" signal
-
-(defund queue3$out-act (inputs st data-width)
-  (b* ((empty-out- (nth 1 inputs))
-       (go-signals (nthcdr (queue3$data-ins-len data-width) inputs))
-       (go-out (nth 3 go-signals))
-
-       (l2 (get-field *queue3$l2* st)))
-    (joint-act (car l2) empty-out- go-out)))
-
-;; Extracting the output data
-
-(defund queue3$data-out (st)
-  (v-threefix (strip-cars (get-field *queue3$d2* st))))
-
-(defthm len-queue3$data-out-1
-  (implies (queue3$st-format st data-width)
-           (equal (len (queue3$data-out st))
-                  data-width))
-  :hints (("Goal" :in-theory (enable queue3$st-format
-                                     queue3$data-out))))
-
-(defthm len-queue3$data-out-2
-  (implies (queue3$valid-st st data-width)
-           (equal (len (queue3$data-out st))
-                  data-width))
-  :hints (("Goal" :in-theory (enable queue3$valid-st))))
-
-(defthm bvp-queue3$data-out
-  (implies (and (queue3$valid-st st data-width)
-                (queue3$out-act inputs st data-width))
-           (bvp (queue3$data-out st)))
-  :hints (("Goal" :in-theory (enable queue3$valid-st
-                                     queue3$out-act
-                                     queue3$data-out))))
-
-(not-primp-lemma queue3)
-
-;; The value lemma for Q3
-
-(defthmd queue3$value
-  (b* ((inputs (list* full-in empty-out- (append data-in go-signals))))
-    (implies (and (queue3& netlist data-width)
-                  (equal (len data-in) data-width)
-                  (true-listp go-signals)
-                  (equal (len go-signals) *queue3$go-num*)
-                  (queue3$st-format st data-width))
-             (equal (se (si 'queue3 data-width) inputs st netlist)
-                    (list* (queue3$in-act inputs st data-width)
-                           (queue3$out-act inputs st data-width)
-                           (queue3$data-out st)))))
-  :hints (("Goal"
-           :do-not-induct t
-           :do-not '(preprocess)
-           :expand (se (si 'queue3 data-width)
-                       (list* full-in empty-out-
-                              (append data-in go-signals))
-                       st
-                       netlist)
-           :in-theory (e/d (de-rules
-                            get-field
-                            len-1-true-listp=>true-listp
-                            not-primp-queue3
-                            queue3&
-                            queue3*$destructure
-                            joint-cntl$value
-                            latch-n$value
-                            v-buf$value
-                            queue3$st-format
-                            queue3$in-act
-                            queue3$out-act
-                            queue3$data-out)
-                           ((queue3*)
-                            de-module-disabled-rules)))))
-
-;; This function specifies the next state of Q3, namely, the next states of three
-;; links L0, L1, and L2.
-
-(defun queue3$state-fn (inputs st data-width)
-  (b* ((data-in    (queue3$data-in inputs data-width))
-       (go-signals (nthcdr (queue3$data-ins-len data-width) inputs))
-
-       (go-trans1 (nth 1 go-signals))
-       (go-trans2 (nth 2 go-signals))
-
-       (l0 (get-field *queue3$l0* st))
-       (d0 (get-field *queue3$d0* st))
-       (l1 (get-field *queue3$l1* st))
-       (d1 (get-field *queue3$d1* st))
-       (l2 (get-field *queue3$l2* st))
-       (d2 (get-field *queue3$d2* st))
-
-       (in-act (queue3$in-act inputs st data-width))
-       (out-act (queue3$out-act inputs st data-width))
-       (trans1-act (joint-act (car l0) (car l1) go-trans1))
-       (trans2-act (joint-act (car l1) (car l2) go-trans2)))
-    (list
-     ;; L0
-     (list (f-sr in-act trans1-act (car l0)))
-     (pairlis$ (fv-if in-act data-in (strip-cars d0))
-               nil)
-
-     ;; L1
-     (list (f-sr trans1-act trans2-act (car l1)))
-     (pairlis$ (fv-if trans1-act (strip-cars d0) (strip-cars d1))
-               nil)
-
-     ;; L2
-     (list (f-sr trans2-act out-act (car l2)))
-     (pairlis$ (fv-if trans2-act (strip-cars d1) (strip-cars d2))
-               nil))))
-
-(defthm len-of-queue3$state-fn
-  (equal (len (queue3$state-fn inputs st data-width))
-         *queue3$st-len*))
-
-;; The state lemma for Q3
-
-(defthmd queue3$state
-  (b* ((inputs (list* full-in empty-out- (append data-in go-signals))))
-    (implies (and (queue3& netlist data-width)
-                  (true-listp data-in)
-                  (equal (len data-in) data-width)
-                  (true-listp go-signals)
-                  (equal (len go-signals) *queue3$go-num*)
-                  (queue3$st-format st data-width))
-             (equal (de (si 'queue3 data-width) inputs st netlist)
-                    (queue3$state-fn inputs st data-width))))
-  :hints (("Goal"
-           :do-not-induct t
-           :do-not '(preprocess)
-           :expand (de (si 'queue3 data-width)
-                       (list* full-in empty-out-
-                              (append data-in go-signals))
-                       st
-                       netlist)
-           :in-theory (e/d (de-rules
-                            get-field
-                            len-1-true-listp=>true-listp
-                            not-primp-queue3
-                            queue3&
-                            queue3*$destructure
-                            queue3$st-format
-                            queue3$data-in
-                            queue3$in-act
-                            queue3$out-act
-                            joint-cntl$value
-                            latch-n$value latch-n$state
-                            v-buf$value)
-                           ((queue3*)
-                            de-module-disabled-rules)))))
-
-(in-theory (disable queue3$state-fn))
-
-;; ======================================================================
-
-;; 2. Specifying the Final State of Q3 After An N-Step Execution
-
 ;; Conditions on the inputs
 
 (defund queue3$input-format (inputs data-width)
@@ -458,27 +457,69 @@
 ;; The extraction function for Q3 that extracts the future output sequence from
 ;; the current state.
 
-(defund queue3$extract-state (st)
+(defund queue3$extract (st)
   (b* ((l0 (get-field *queue3$l0* st))
        (d0 (get-field *queue3$d0* st))
        (l1 (get-field *queue3$l1* st))
        (d1 (get-field *queue3$d1* st))
        (l2 (get-field *queue3$l2* st))
        (d2 (get-field *queue3$d2* st)))
-    (extract-state (list l0 d0 l1 d1 l2 d2))))
+    (extract-valid-data (list l0 d0 l1 d1 l2 d2))))
 
-(defthm queue3$extract-state-not-empty
+(defthm queue3$extract-not-empty
   (implies (and (queue3$out-act inputs st data-width)
                 (queue3$valid-st st data-width))
-           (< 0 (len (queue3$extract-state st))))
+           (< 0 (len (queue3$extract st))))
   :hints (("Goal"
            :in-theory (e/d (queue3$valid-st
-                            queue3$extract-state
+                            queue3$extract
                             queue3$out-act)
                            (nfix))))
   :rule-classes :linear)
 
-;; Extracting the accepted input sequence
+;; The extracted next-state function for Q3.  Note that this function avoids
+;; exploring the internal computation of Q3.
+
+(defund queue3$extracted-step (inputs st data-width)
+  (b* ((data-in (queue3$data-in inputs data-width))
+       (extracted-st (queue3$extract st))
+       (n (1- (len extracted-st))))
+    (cond
+     ((equal (queue3$out-act inputs st data-width) t)
+      (cond
+       ((equal (queue3$in-act inputs st data-width) t)
+        (cons data-in (take n extracted-st)))
+       (t (take n extracted-st))))
+     (t (cond
+         ((equal (queue3$in-act inputs st data-width) t)
+          (cons data-in extracted-st))
+         (t extracted-st))))))
+
+;; The single-step-update property
+
+(defthm queue3$extracted-step-correct
+  (b* ((next-st (queue3$step inputs st data-width)))
+    (implies (and (queue3$input-format inputs data-width)
+                  (queue3$valid-st st data-width))
+             (equal (queue3$extract next-st)
+                    (queue3$extracted-step inputs st data-width))))
+  :hints (("Goal"
+           :in-theory (enable get-field
+                              f-sr
+                              queue3$extracted-step
+                              queue3$input-format
+                              queue3$valid-st
+                              queue3$st-format
+                              queue3$step
+                              queue3$in-act
+                              queue3$out-act
+                              queue3$extract))))
+
+;; ======================================================================
+
+;; 4. Relationship Between the Input and Output Sequences
+
+;; Extract the accepted input sequence
 
 (defun queue3$in-seq (inputs-lst st data-width n)
   (declare (xargs :measure (acl2-count n)))
@@ -487,16 +528,16 @@
     (b* ((inputs (car inputs-lst)))
       (if (equal (queue3$in-act inputs st data-width) t)
           (append (queue3$in-seq (cdr inputs-lst)
-                                 (queue3$state-fn inputs st data-width)
+                                 (queue3$step inputs st data-width)
                                  data-width
                                  (1- n))
                   (list (queue3$data-in inputs data-width)))
         (queue3$in-seq (cdr inputs-lst)
-                       (queue3$state-fn inputs st data-width)
+                       (queue3$step inputs st data-width)
                        data-width
                        (1- n))))))
 
-;; Extracting the valid output sequence
+;; Extract the valid output sequence
 
 (defun queue3$out-seq (inputs-lst st data-width n)
   (declare (xargs :measure (acl2-count n)))
@@ -505,12 +546,12 @@
     (b* ((inputs (car inputs-lst)))
       (if (equal (queue3$out-act inputs st data-width) t)
           (append (queue3$out-seq (cdr inputs-lst)
-                                  (queue3$state-fn inputs st data-width)
+                                  (queue3$step inputs st data-width)
                                   data-width
                                   (1- n))
                   (list (queue3$data-out st)))
         (queue3$out-seq (cdr inputs-lst)
-                        (queue3$state-fn inputs st data-width)
+                        (queue3$step inputs st data-width)
                         data-width
                         (1- n))))))
 
@@ -539,60 +580,19 @@
                    (queue3$out-seq inputs-lst st data-width n)))))
      state)))
 
-;; The extracted next-state function for Q3
-
-(defund queue3$step-spec (inputs st data-width)
-  (b* ((data-in (queue3$data-in inputs data-width))
-       (extracted-st (queue3$extract-state st))
-       (n (1- (len extracted-st))))
-    (cond
-     ((equal (queue3$out-act inputs st data-width) t)
-      (cond
-       ((equal (queue3$in-act inputs st data-width) t)
-        (cons data-in (take n extracted-st)))
-       (t (take n extracted-st))))
-     (t (cond
-         ((equal (queue3$in-act inputs st data-width) t)
-          (cons data-in extracted-st))
-         (t extracted-st))))))
-
-;; The single-step-update property
-
-(defthm queue3$step-spec-correct
-  (b* ((next-st (queue3$state-fn inputs st data-width)))
-    (implies (and (queue3$input-format inputs data-width)
-                  (queue3$valid-st st data-width))
-             (equal (queue3$extract-state next-st)
-                    (queue3$step-spec inputs st data-width))))
-  :hints (("Goal"
-           :in-theory (enable get-field
-                              f-sr
-                              queue3$step-spec
-                              queue3$input-format
-                              queue3$valid-st
-                              queue3$st-format
-                              queue3$state-fn
-                              queue3$in-act
-                              queue3$out-act
-                              queue3$extract-state))))
-
-;; ======================================================================
-
-;; 4. Relationship Between the Input and Output Sequences
-
-;; Proving that queue3$valid-st is an invariant.
+;; Prove that queue3$valid-st is an invariant.
 
 (defthm queue3$valid-st-preserved
   (implies (and (queue3$input-format inputs data-width)
                 (queue3$valid-st st data-width))
-           (queue3$valid-st (queue3$state-fn inputs st data-width)
+           (queue3$valid-st (queue3$step inputs st data-width)
                             data-width))
   :hints (("Goal"
            :in-theory (e/d (get-field
                             queue3$input-format
                             queue3$valid-st
                             queue3$st-format
-                            queue3$state-fn
+                            queue3$step
                             queue3$in-act
                             queue3$out-act
                             f-sr)
@@ -600,18 +600,18 @@
                             nthcdr
                             acl2::true-listp-append)))))
 
-(defthm queue3$extract-state-lemma
+(defthm queue3$extract-lemma
   (implies (and (queue3$valid-st st data-width)
-                (equal n (1- (len (queue3$extract-state st))))
+                (equal n (1- (len (queue3$extract st))))
                 (queue3$out-act inputs st data-width))
            (equal (append
-                   (take n (queue3$extract-state st))
+                   (take n (queue3$extract st))
                    (list (queue3$data-out st)))
-                  (queue3$extract-state st)))
+                  (queue3$extract st)))
   :hints (("Goal"
            :in-theory (enable queue3$valid-st
                               queue3$st-format
-                              queue3$extract-state
+                              queue3$extract
                               queue3$out-act
                               queue3$data-out))))
 
